src/goose_lang/proofmode.v
@@ -3,7 +3,7 @@ From iris.proofmode Require Export environments.
 From Perennial.Helpers Require Export ipm.
 From Perennial.program_logic Require Export weakestpre.
 From Perennial.program_logic Require Import atomic.
-From Perennial.goose_lang Require Export lifting.
+From Perennial.goose_lang Require Export lang lifting.
 From Perennial.goose_lang Require Export typing.
 Set Default Proof Using "Type".
 Import uPred.
